src/Shallow/SeqDiskProg.v
@@ -7,7 +7,8 @@ Module D.
 
   Inductive Op : Type -> Type :=
   | Read (a:addr) : Op block
-  | Write (a:addr) (b:block) : Op unit.
+  | Write (a:addr) (b:block) : Op unit
+  | DiskSize : Op nat.
 
   Definition prog := Prog.prog Op.
 
@@ -19,7 +20,9 @@ Module D.
       step (Read a) state b state
   | step_write : forall a b0 b (state: State),
       state a = Some b0 ->
-      step (Write a b) state tt (diskUpd state a b).
+      step (Write a b) state tt (diskUpd state a b)
+  | step_disk_size : forall (state: State),
+      step (DiskSize) state (size state) state.
 
   Definition exec := Prog.exec step.
   Definition exec_recover := Prog.exec_recover step.
