src/Shallow/TwoDiskProgTheorems.v
@@ -144,7 +144,67 @@ Proof.
     repeat (destruct matches in *; cleanup).
 Qed.
 
+Theorem TDDiskSize0_ok :
+    prog_ok
+      (fun '(d_0, F) state =>
+         {|
+           pre := TD.disk0 state |= eq d_0 /\
+                  TD.disk1 state |= F;
+           post :=
+             fun r state' =>
+               match r with
+               | Working n => n = size d_0 /\
+                             TD.disk0 state' |= eq d_0 /\
+                             TD.disk1 state' |= F
+               | Failed => TD.disk0 state' |= [|False|] /\
+                          TD.disk1 state' |= F
+               end;
+           crash :=
+             fun state' =>
+               TD.disk0 state' |= eq d_0 /\
+               TD.disk1 state' |= F;
+         |})
+      (Prim (TD.DiskSize d0))
+      TD.step.
+Proof.
+  start_prim.
+  TD.inv_step; simpl.
+  TD.inv_bg; cleanup;
+    repeat (destruct matches in *; cleanup).
+Qed.
+
+Theorem TDDiskSize1_ok :
+    prog_ok
+      (fun '(F, d_1) state =>
+         {|
+           pre := TD.disk0 state |= F /\
+                  TD.disk1 state |= eq d_1;
+           post :=
+             fun r state' =>
+               match r with
+               | Working n => n = size d_1 /\
+                             TD.disk0 state' |= F /\
+                             TD.disk1 state' |= eq d_1
+               | Failed => TD.disk0 state' |= F /\
+                          TD.disk1 state' |= [|False|]
+               end;
+           crash :=
+             fun state' =>
+               TD.disk0 state' |= F /\
+               TD.disk1 state' |= eq d_1;
+         |})
+      (Prim (TD.DiskSize d1))
+      TD.step.
+Proof.
+  start_prim.
+  TD.inv_step; simpl.
+  TD.inv_bg; cleanup;
+    repeat (destruct matches in *; cleanup).
+Qed.
+
 Hint Extern 1 {{ Prim (TD.Read d0 _); _}} => apply TDRead0_ok : prog.
 Hint Extern 1 {{ Prim (TD.Read d1 _); _}} => apply TDRead1_ok : prog.
 Hint Extern 1 {{ Prim (TD.Write d0 _ _); _}} => apply TDWrite0_ok : prog.
 Hint Extern 1 {{ Prim (TD.Write d1 _ _); _}} => apply TDWrite1_ok : prog.
+Hint Extern 1 {{ Prim (TD.DiskSize d0); _}} => apply TDDiskSize0_ok : prog.
+Hint Extern 1 {{ Prim (TD.DiskSize d1); _}} => apply TDDiskSize1_ok : prog.
